src/Mail2/MailFSPathAbsImpl.v
@@ -1,39 +1,61 @@
 Require Import POCS.
 Require Import String.
 Require Import MailServerAPI.
-Require Import MailServerDirAPI.
-Require Import MailboxTmpAbsAPI.
-Require Import MailFSAPI.
+Require Import MailFSStringAbsAPI.
+Require Import MailFSStringAPI.
 Require Import MailFSPathAbsAPI.
 
-Import ListNotations.
-Open Scope string.
 
-Module MailFSPathAbsImpl <: LayerImpl MailFSPathAbsAPI MailFSAPI.
+Module MailFSPathAbsImpl <: LayerImpl MailFSPathAbsAPI MailFSStringAPI.
 
-  Definition absR (s1 : MailFSPathAbsAPI.State) (s2 : MailFSAPI.State) := 
-    forall tid fn, FMap.In ("tmp", (tid, fn)) s1 <-> FMap.In (tid, fn) (MailboxTmpAbsAPI.tmpdir s2) /\
-              FMap.In ("maildir", (tid, fn)) s1 <-> FMap.In (tid, fn) (MailboxTmpAbsAPI.maildir s2).
-                                              
-  Definition compile_ts (ts : @threads_state MailFSAPI.opT) := ts.
+  Definition absR (s1 : MailFSPathAbsAPI.State) (s2 : MailFSStringAPI.State) :=
+    forall dirname filename contents,
+      FMap.MapsTo (dirname, filename) contents s1 <->
+      ( dirname = "tmp"%string /\ FMap.MapsTo filename contents (MailFSStringAbsAPI.tmpdir s2) \/
+        dirname = "mail"%string /\ FMap.MapsTo filename contents (MailFSStringAbsAPI.maildir s2) ).
+
+  Definition compile_ts (ts : @threads_state MailFSStringAPI.opT) := ts.
 
   Theorem compile_ts_no_atomics :
-    forall (ts : @threads_state MailFSAPI.opT),
+    forall (ts : @threads_state MailFSStringAPI.opT),
       no_atomics_ts ts ->
       no_atomics_ts (compile_ts ts).
   Proof.
     unfold compile_ts; eauto.
   Qed.
 
-  Hint Extern 1 (MailFSAPI.step _ _ _ _ _ _) => econstructor.
+  Hint Extern 1 (MailFSStringAPI.step _ _ _ _ _ _) => econstructor.
+
+  Lemma fn_ne : forall (dirname fn1 fn2 : string),
+    (dirname, fn1) <> (dirname, fn2) ->
+    fn1 <> fn2.
+  Proof.
+    congruence.
+  Qed.
+
+  Hint Resolve FMap.add_mapsto.
+  Hint Resolve FMap.mapsto_add_ne'.
+  Hint Resolve fn_ne.
 
   Theorem absR_ok :
-    op_abs absR MailFSPathAbsAPI.step MailFSAPI.step.
+    op_abs absR MailFSPathAbsAPI.step MailFSStringAPI.step.
   Proof.
-    unfold op_abs, absR; intros.
-    destruct s1; simpl in *; subst.
+    unfold op_abs; intros.
+    destruct s2; simpl in *; subst.
     inversion H0; clear H0; subst; repeat sigT_eq.
+    all: eexists.
+    all: split; [ | econstructor ].
+    all: simpl.
     all: eauto 10.
+
+(*
+    split; intros.
+    eapply FMap.mapsto_add_or in H0; intuition idtac; subst.
+    inversion H0; clear H0; subst.
+    eauto.
+    eapply H in H3.
+    intuition ( subst; eauto ).
+*)
   Admitted.
 
   Hint Resolve absR_ok.
@@ -44,7 +66,7 @@ Module MailFSPathAbsImpl <: LayerImpl MailFSPathAbsAPI MailFSAPI.
       traces_match_abs absR
         MailFSPathAbsAPI.initP
         MailFSPathAbsAPI.step
-        MailFSAPI.step (compile_ts ts) ts.
+        MailFSStringAPI.step (compile_ts ts) ts.
   Proof.
     unfold compile_ts, traces_match_abs; intros.
     eexists; intuition idtac.
@@ -56,11 +78,9 @@ Module MailFSPathAbsImpl <: LayerImpl MailFSPathAbsAPI MailFSAPI.
     forall s1 s2,
       MailFSPathAbsAPI.initP s1 ->
       absR s1 s2 ->
-      MailFSAPI.initP s2.
+      MailFSStringAPI.initP s2.
   Proof.
     eauto.
   Qed.
-  
-
 
 End MailFSPathAbsImpl.
