src/Mail2/MailFSPathAPI.v
@@ -1,0 +1,89 @@
+Require Import POCS.
+Require Import String.
+Require Import MailServerAPI.
+Require Import MailFSPathAbsAPI.
+
+
+Module MailFSPathAPI <: Layer.
+
+  Import MailServerAPI.
+  Import MailFSPathAbsAPI.
+
+  Inductive xopT : Type -> Type :=
+  | CreateWrite : forall (tmpfn : string * string) (data : string), xopT unit
+  | Link : forall (tmpfn : string * string) (mboxfn : string * string), xopT unit
+  | Unlink : forall (tmpfn : string * string), xopT unit
+
+  | GetTID : xopT nat
+  | List : forall (dir : string), xopT (list string)
+  | Read : forall (fn : string * string), xopT string
+  | GetRequest : xopT request
+  | Respond : forall (T : Type) (v : T), xopT unit
+  .
+
+  Definition opT := xopT.
+  Definition State := MailFSPathAbsAPI.State.
+  Definition initP (s : State) := True.
+
+  Inductive xstep : forall T, opT T -> nat -> State -> T -> State -> list event -> Prop :=
+  | StepCreateWrite : forall fs tid tmpfn data,
+    ~ FMap.In tmpfn fs ->
+    xstep (CreateWrite tmpfn data) tid
+      fs
+      tt
+      (FMap.add tmpfn data fs)
+      nil
+  | StepUnlink : forall fs tid tmpfn,
+    xstep (Unlink tmpfn) tid
+      fs
+      tt
+      (FMap.remove tmpfn fs)
+      nil
+  | StepLink : forall fs tid mailfn data tmpfn,
+    FMap.MapsTo tmpfn data fs ->
+    ~ FMap.In mailfn fs ->
+    xstep (Link tmpfn mailfn) tid
+      fs
+      tt
+      (FMap.add mailfn data fs)
+      nil
+
+  | StepList : forall fs tid r dirname,
+    FMap.is_permutation_key r (drop_dirname (filter_dir dirname fs)) ->
+    xstep (List dirname) tid
+      fs
+      r
+      fs
+      nil
+
+  | StepGetTID : forall fs tid,
+    xstep GetTID tid
+      fs
+      tid
+      fs
+      nil
+
+  | StepRead : forall fn fs tid m,
+    FMap.MapsTo fn m fs ->
+    xstep (Read fn) tid
+      fs
+      m
+      fs
+      nil
+  | StepGetRequest : forall s tid r,
+    xstep GetRequest tid
+      s
+      r
+      s
+      (Event r :: nil)
+  | StepRespond : forall s tid T (v : T),
+    xstep (Respond v) tid
+      s
+      tt
+      s
+      (Event v :: nil)
+  .
+
+  Definition step := xstep.
+
+End MailFSPathAPI.
