src/Mail2/MailFSPathImpl.v
@@ -1,0 +1,243 @@
+Require Import POCS.
+Require Import String.
+Require Import MailServerAPI.
+Require Import MailFSStringAPI.
+Require Import MailFSPathAbsAPI.
+Require Import MailFSPathAPI.
+
+
+Module MailFSPathImpl <: LayerImpl MailFSPathAPI MailFSPathAbsAPI.
+
+  Definition createwritetmp_core fn data :=
+    r <- Op (MailFSPathAPI.CreateWrite ("tmp"%string, fn) data);
+    Ret r.
+
+  Definition linkmail_core tmpfn mboxfn :=
+    v <- Op (MailFSPathAPI.Link ("tmp"%string, tmpfn) ("mail"%string, mboxfn));
+    Ret v.
+
+  Definition unlinktmp_core tmpfn :=
+    r <- Op (MailFSPathAPI.Unlink ("tmp"%string, tmpfn));
+    Ret r.
+
+  Definition gettid_core :=
+    r <- Op (MailFSPathAPI.GetTID);
+    Ret r.
+
+  Definition list_core :=
+    l <- Op (MailFSPathAPI.List "mail"%string);
+    Ret l.
+
+  Definition read_core (fn : string) :=
+    r <- Op (MailFSPathAPI.Read ("mail"%string, fn));
+    Ret r.
+
+  Definition getrequest_core :=
+    r <- Op (MailFSPathAPI.GetRequest);
+    Ret r.
+
+  Definition respond_core T (r : T) :=
+    r <- Op (MailFSPathAPI.Respond r);
+    Ret r.
+
+  Definition compile_op T (op : MailFSPathAbsAPI.opT T) : proc _ T :=
+    match op with
+    | MailFSStringAPI.LinkMail tmpfn mailfn => linkmail_core tmpfn mailfn
+    | MailFSStringAPI.List => list_core
+    | MailFSStringAPI.Read fn => read_core fn
+    | MailFSStringAPI.CreateWriteTmp tmpfn data => createwritetmp_core tmpfn data
+    | MailFSStringAPI.UnlinkTmp tmpfn => unlinktmp_core tmpfn
+    | MailFSStringAPI.GetRequest => getrequest_core
+    | MailFSStringAPI.Respond r => respond_core r
+    | MailFSStringAPI.GetTID => gettid_core
+    end.
+
+  Ltac step_inv :=
+    match goal with
+    | H : MailFSPathAbsAPI.step _ _ _ _ _ _ |- _ =>
+      inversion H; clear H; subst; repeat sigT_eq
+    | H : MailFSPathAPI.step _ _ _ _ _ _ |- _ =>
+      inversion H; clear H; subst; repeat sigT_eq
+    end; intuition idtac.
+
+  Hint Extern 1 (MailFSPathAbsAPI.step _ _ _ _ _ _) => econstructor.
+  Hint Extern 1 (MailFSPathAPI.step _ _ _ _ _ _) => econstructor.
+
+  Theorem linkmail_atomic : forall `(rx : _ -> proc _ T) fn m,
+    trace_incl MailFSPathAPI.step
+      (Bind (compile_op (MailFSStringAPI.LinkMail fn m)) rx)
+      (Bind (atomize compile_op (MailFSStringAPI.LinkMail fn m)) rx).
+  Proof.
+    intros.
+    eapply trace_incl_atomize_ysa.
+    simpl.
+    unfold linkmail_core, ysa_movers.
+    eauto 20.
+  Qed.
+
+  Theorem list_atomic : forall `(rx : _ -> proc _ T),
+    trace_incl MailFSPathAPI.step
+      (Bind (compile_op (MailFSStringAPI.List)) rx)
+      (Bind (atomize compile_op (MailFSStringAPI.List)) rx).
+  Proof.
+    intros.
+    eapply trace_incl_atomize_ysa.
+    simpl.
+    unfold list_core, ysa_movers.
+    eauto 20.
+  Qed.
+
+  Theorem read_atomic : forall `(rx : _ -> proc _ T) fn,
+    trace_incl MailFSPathAPI.step
+      (Bind (compile_op (MailFSStringAPI.Read fn)) rx)
+      (Bind (atomize compile_op (MailFSStringAPI.Read fn)) rx).
+  Proof.
+    intros.
+    eapply trace_incl_atomize_ysa.
+    simpl.
+    unfold read_core, ysa_movers.
+    eauto 20.
+  Qed.
+
+  Theorem createwritetmp_atomic : forall `(rx : _ -> proc _ T) tmpfn data,
+    trace_incl MailFSPathAPI.step
+      (Bind (compile_op (MailFSStringAPI.CreateWriteTmp tmpfn data)) rx)
+      (Bind (atomize compile_op (MailFSStringAPI.CreateWriteTmp tmpfn data)) rx).
+  Proof.
+    intros.
+    eapply trace_incl_atomize_ysa.
+    simpl.
+    unfold createwritetmp_core, ysa_movers.
+    eauto 20.
+  Qed.
+
+  Theorem unlinktmp_atomic : forall `(rx : _ -> proc _ T) fn,
+    trace_incl MailFSPathAPI.step
+      (Bind (compile_op (MailFSStringAPI.UnlinkTmp fn)) rx)
+      (Bind (atomize compile_op (MailFSStringAPI.UnlinkTmp fn)) rx).
+  Proof.
+    intros.
+    eapply trace_incl_atomize_ysa.
+    simpl.
+    unfold unlinktmp_core, ysa_movers.
+    eauto 20.
+  Qed.
+
+  Theorem gettid_atomic : forall `(rx : _ -> proc _ T),
+    trace_incl MailFSPathAPI.step
+      (Bind (compile_op (MailFSStringAPI.GetTID)) rx)
+      (Bind (atomize compile_op (MailFSStringAPI.GetTID)) rx).
+  Proof.
+    intros.
+    eapply trace_incl_atomize_ysa.
+    simpl.
+    unfold gettid_core, ysa_movers.
+    eauto 20.
+  Qed.
+
+  Theorem getrequest_atomic : forall `(rx : _ -> proc _ T),
+    trace_incl MailFSPathAPI.step
+      (Bind (compile_op (MailFSStringAPI.GetRequest)) rx)
+      (Bind (atomize compile_op (MailFSStringAPI.GetRequest)) rx).
+  Proof.
+    intros.
+    eapply trace_incl_atomize_ysa.
+    simpl.
+    unfold getrequest_core, ysa_movers.
+    eauto 20.
+  Qed.
+
+  Theorem respond_atomic : forall `(rx : _ -> proc _ T) Tr (r : Tr),
+    trace_incl MailFSPathAPI.step
+      (Bind (compile_op (MailFSStringAPI.Respond r)) rx)
+      (Bind (atomize compile_op (MailFSStringAPI.Respond r)) rx).
+  Proof.
+    intros.
+    eapply trace_incl_atomize_ysa.
+    simpl.
+    unfold respond_core, ysa_movers.
+    eauto 20.
+  Qed.
+
+  Theorem my_compile_correct :
+    compile_correct compile_op MailFSPathAPI.step MailFSPathAbsAPI.step.
+  Proof.
+    unfold compile_correct; intros.
+    destruct op.
+
+    all: try solve [ repeat atomic_exec_inv; repeat step_inv; eauto ].
+  Qed.
+
+  Theorem my_atomize_correct :
+    atomize_correct compile_op MailFSPathAPI.step.
+  Proof.
+    unfold atomize_correct; intros.
+    destruct op.
+    + rewrite createwritetmp_atomic.
+      eapply trace_incl_bind_a; eauto.
+    + rewrite linkmail_atomic.
+      eapply trace_incl_bind_a; eauto.
+    + rewrite unlinktmp_atomic.
+      eapply trace_incl_bind_a; eauto.
+    + rewrite gettid_atomic.
+      eapply trace_incl_bind_a; eauto.
+    + rewrite list_atomic.
+      eapply trace_incl_bind_a; eauto.
+    + rewrite read_atomic.
+      eapply trace_incl_bind_a; eauto.
+    + rewrite getrequest_atomic.
+      eapply trace_incl_bind_a; eauto.
+    + rewrite respond_atomic.
+      eapply trace_incl_bind_a; eauto.
+  Qed.
+
+  Hint Resolve my_compile_correct.
+  Hint Resolve my_atomize_correct.
+
+  Theorem all_traces_match :
+    forall ts1 ts2,
+      proc_match (Compile.compile_ok compile_op) ts1 ts2 ->
+      traces_match_ts MailFSPathAPI.step MailFSPathAbsAPI.step ts1 ts2.
+  Proof.
+    intros.
+    eapply Compile.compile_traces_match_ts; eauto.
+  Qed.
+
+  Definition absR (s1 : MailFSPathAPI.State) (s2 : MailFSPathAbsAPI.State) :=
+    s1 = s2.
+
+  Definition compile_ts := Compile.compile_ts compile_op.
+
+  Theorem compile_ts_no_atomics :
+    forall ts,
+      no_atomics_ts ts ->
+      no_atomics_ts (compile_ts ts).
+  Proof.
+    eapply Compile.compile_ts_no_atomics.
+    destruct op; compute; eauto.
+  Qed.
+
+  Theorem compile_traces_match :
+    forall ts2,
+      no_atomics_ts ts2 ->
+      traces_match_abs absR
+        MailFSPathAPI.initP
+        MailFSPathAPI.step
+        MailFSPathAbsAPI.step (compile_ts ts2) ts2.
+  Proof.
+    unfold traces_match_abs; intros.
+    rewrite H2 in *; clear H2.
+    eapply all_traces_match; eauto.
+    eapply Compile.compile_ts_ok; eauto.
+  Qed.
+
+  Theorem absInitP :
+    forall s1 s2,
+      MailFSPathAPI.initP s1 ->
+      absR s1 s2 ->
+      MailFSPathAbsAPI.initP s2.
+  Proof.
+    eauto.
+  Qed.
+
+End MailFSPathImpl.
