src/Mail2/MailFSStringImpl.v
@@ -1,0 +1,264 @@
+Require Import POCS.
+Require Import String.
+Require Import MailServerAPI.
+Require Import MailFSAPI.
+Require Import MailFSStringAPI.
+Require Import MailFSStringAbsAPI.
+
+
+Module MailFSStringImpl <: LayerImpl MailFSStringAPI MailFSStringAbsAPI.
+
+  Definition createwritetmp_core data :=
+    tid <- Op (MailFSStringAPI.GetTID);
+    r <- Op (MailFSStringAPI.CreateWriteTmp (encode_tid_fn tid ""%string) data);
+    Ret r.
+
+  Definition linkmail_core mboxfn :=
+    tid <- Op (MailFSStringAPI.GetTID);
+    v <- Op (MailFSStringAPI.LinkMail (encode_tid_fn tid ""%string) (encode_tid_fn tid mboxfn));
+    Ret v.
+
+  Definition unlinktmp_core :=
+    tid <- Op (MailFSStringAPI.GetTID);
+    r <- Op (MailFSStringAPI.UnlinkTmp (encode_tid_fn tid ""%string));
+    Ret r.
+
+  Definition gettid_core :=
+    r <- Op (MailFSStringAPI.GetTID);
+    Ret r.
+
+  Definition list_core :=
+    l <- Op (MailFSStringAPI.List);
+    Ret (map decode_tid_fn l).
+
+  Definition read_core (fn : nat*string) :=
+    r <- Op (MailFSStringAPI.Read (encode_tid_fn (fst fn) (snd fn)));
+    Ret r.
+
+  Definition getrequest_core :=
+    r <- Op (MailFSStringAPI.GetRequest);
+    Ret r.
+
+  Definition respond_core T (r : T) :=
+    r <- Op (MailFSStringAPI.Respond r);
+    Ret r.
+
+  Definition compile_op T (op : MailFSStringAbsAPI.opT T) : proc _ T :=
+    match op with
+    | MailFSAPI.LinkMail m => linkmail_core m
+    | MailFSAPI.List => list_core
+    | MailFSAPI.Read fn => read_core fn
+    | MailFSAPI.CreateWriteTmp data => createwritetmp_core data
+    | MailFSAPI.UnlinkTmp => unlinktmp_core
+    | MailFSAPI.GetRequest => getrequest_core
+    | MailFSAPI.Respond r => respond_core r
+    | MailFSAPI.GetTID => gettid_core
+    end.
+
+  Ltac step_inv :=
+    match goal with
+    | H : MailFSStringAbsAPI.step _ _ _ _ _ _ |- _ =>
+      inversion H; clear H; subst; repeat sigT_eq
+    | H : MailFSStringAPI.step _ _ _ _ _ _ |- _ =>
+      inversion H; clear H; subst; repeat sigT_eq
+    end; intuition idtac.
+
+  Hint Extern 1 (MailFSStringAbsAPI.step _ _ _ _ _ _) => econstructor.
+  Hint Extern 1 (MailFSStringAPI.step _ _ _ _ _ _) => econstructor.
+
+  Lemma gettid_right_mover :
+    right_mover
+      MailFSStringAPI.step
+      (MailFSStringAPI.GetTID).
+  Proof.
+    unfold right_mover; intros.
+    repeat step_inv; eauto.
+  Qed.
+
+  Hint Resolve gettid_right_mover.
+
+  Theorem linkmail_atomic : forall `(rx : _ -> proc _ T) m,
+    trace_incl MailFSStringAPI.step
+      (Bind (compile_op (MailFSAPI.LinkMail m)) rx)
+      (Bind (atomize compile_op (MailFSAPI.LinkMail m)) rx).
+  Proof.
+    intros.
+    eapply trace_incl_atomize_ysa.
+    simpl.
+    unfold linkmail_core, ysa_movers.
+    eauto 20.
+  Qed.
+
+  Theorem list_atomic : forall `(rx : _ -> proc _ T),
+    trace_incl MailFSStringAPI.step
+      (Bind (compile_op (MailFSAPI.List)) rx)
+      (Bind (atomize compile_op (MailFSAPI.List)) rx).
+  Proof.
+    intros.
+    eapply trace_incl_atomize_ysa.
+    simpl.
+    unfold list_core, ysa_movers.
+    eauto 20.
+  Qed.
+
+  Theorem read_atomic : forall `(rx : _ -> proc _ T) fn,
+    trace_incl MailFSStringAPI.step
+      (Bind (compile_op (MailFSAPI.Read fn)) rx)
+      (Bind (atomize compile_op (MailFSAPI.Read fn)) rx).
+  Proof.
+    intros.
+    eapply trace_incl_atomize_ysa.
+    simpl.
+    unfold read_core, ysa_movers.
+    eauto 20.
+  Qed.
+
+  Theorem createwritetmp_atomic : forall `(rx : _ -> proc _ T) fn,
+    trace_incl MailFSStringAPI.step
+      (Bind (compile_op (MailFSAPI.CreateWriteTmp fn)) rx)
+      (Bind (atomize compile_op (MailFSAPI.CreateWriteTmp fn)) rx).
+  Proof.
+    intros.
+    eapply trace_incl_atomize_ysa.
+    simpl.
+    unfold createwritetmp_core, ysa_movers.
+    eauto 20.
+  Qed.
+
+  Theorem unlinktmp_atomic : forall `(rx : _ -> proc _ T),
+    trace_incl MailFSStringAPI.step
+      (Bind (compile_op (MailFSAPI.UnlinkTmp)) rx)
+      (Bind (atomize compile_op (MailFSAPI.UnlinkTmp)) rx).
+  Proof.
+    intros.
+    eapply trace_incl_atomize_ysa.
+    simpl.
+    unfold unlinktmp_core, ysa_movers.
+    eauto 20.
+  Qed.
+
+  Theorem gettid_atomic : forall `(rx : _ -> proc _ T),
+    trace_incl MailFSStringAPI.step
+      (Bind (compile_op (MailFSAPI.GetTID)) rx)
+      (Bind (atomize compile_op (MailFSAPI.GetTID)) rx).
+  Proof.
+    intros.
+    eapply trace_incl_atomize_ysa.
+    simpl.
+    unfold gettid_core, ysa_movers.
+    eauto 20.
+  Qed.
+
+  Theorem getrequest_atomic : forall `(rx : _ -> proc _ T),
+    trace_incl MailFSStringAPI.step
+      (Bind (compile_op (MailFSAPI.GetRequest)) rx)
+      (Bind (atomize compile_op (MailFSAPI.GetRequest)) rx).
+  Proof.
+    intros.
+    eapply trace_incl_atomize_ysa.
+    simpl.
+    unfold getrequest_core, ysa_movers.
+    eauto 20.
+  Qed.
+
+  Theorem respond_atomic : forall `(rx : _ -> proc _ T) Tr (r : Tr),
+    trace_incl MailFSStringAPI.step
+      (Bind (compile_op (MailFSAPI.Respond r)) rx)
+      (Bind (atomize compile_op (MailFSAPI.Respond r)) rx).
+  Proof.
+    intros.
+    eapply trace_incl_atomize_ysa.
+    simpl.
+    unfold respond_core, ysa_movers.
+    eauto 20.
+  Qed.
+
+  Theorem my_compile_correct :
+    compile_correct compile_op MailFSStringAPI.step MailFSStringAbsAPI.step.
+  Proof.
+    unfold compile_correct; intros.
+    destruct op.
+
+    all: try solve [ repeat atomic_exec_inv; repeat step_inv; eauto ].
+
+    repeat atomic_exec_inv.
+    repeat step_inv; eauto.
+    simpl.
+
+    destruct fn; simpl in *.
+    eauto.
+  Qed.
+
+  Theorem my_atomize_correct :
+    atomize_correct compile_op MailFSStringAPI.step.
+  Proof.
+    unfold atomize_correct; intros.
+    destruct op.
+    + rewrite createwritetmp_atomic.
+      eapply trace_incl_bind_a; eauto.
+    + rewrite linkmail_atomic.
+      eapply trace_incl_bind_a; eauto.
+    + rewrite unlinktmp_atomic.
+      eapply trace_incl_bind_a; eauto.
+    + rewrite gettid_atomic.
+      eapply trace_incl_bind_a; eauto.
+    + rewrite list_atomic.
+      eapply trace_incl_bind_a; eauto.
+    + rewrite read_atomic.
+      eapply trace_incl_bind_a; eauto.
+    + rewrite getrequest_atomic.
+      eapply trace_incl_bind_a; eauto.
+    + rewrite respond_atomic.
+      eapply trace_incl_bind_a; eauto.
+  Qed.
+
+  Hint Resolve my_compile_correct.
+  Hint Resolve my_atomize_correct.
+
+  Theorem all_traces_match :
+    forall ts1 ts2,
+      proc_match (Compile.compile_ok compile_op) ts1 ts2 ->
+      traces_match_ts MailFSStringAPI.step MailFSStringAbsAPI.step ts1 ts2.
+  Proof.
+    intros.
+    eapply Compile.compile_traces_match_ts; eauto.
+  Qed.
+
+  Definition absR (s1 : MailFSStringAPI.State) (s2 : MailFSStringAbsAPI.State) :=
+    s1 = s2.
+
+  Definition compile_ts := Compile.compile_ts compile_op.
+
+  Theorem compile_ts_no_atomics :
+    forall ts,
+      no_atomics_ts ts ->
+      no_atomics_ts (compile_ts ts).
+  Proof.
+    eapply Compile.compile_ts_no_atomics.
+    destruct op; compute; eauto.
+  Qed.
+
+  Theorem compile_traces_match :
+    forall ts2,
+      no_atomics_ts ts2 ->
+      traces_match_abs absR
+        MailFSStringAPI.initP
+        MailFSStringAPI.step
+        MailFSStringAbsAPI.step (compile_ts ts2) ts2.
+  Proof.
+    unfold traces_match_abs; intros.
+    rewrite H2 in *; clear H2.
+    eapply all_traces_match; eauto.
+    eapply Compile.compile_ts_ok; eauto.
+  Qed.
+
+  Theorem absInitP :
+    forall s1 s2,
+      MailFSStringAPI.initP s1 ->
+      absR s1 s2 ->
+      MailFSStringAbsAPI.initP s2.
+  Proof.
+    eauto.
+  Qed.
+
+End MailFSStringImpl.
